Finished player_tangle_attractor_I_step
Might need cleanup/simplification.

TangleLearning.thy
@@ -536,7 +536,8 @@ begin
     | escape: "\<lbrakk>t \<in> T; t-S \<noteq> {}; opponent_escapes t \<noteq> {}; opponent_escapes t \<subseteq> S; A \<subseteq> S\<rbrakk>
                     \<Longrightarrow> attractor_step S (S \<union> t)"
 
-    definition a :: "'v set \<Rightarrow> bool" where "a \<equiv> attractor_step\<^sup>*\<^sup>* A"
+    definition is_player_tangle_attractor :: "'v set \<Rightarrow> bool" where
+      "is_player_tangle_attractor \<equiv> attractor_step\<^sup>*\<^sup>* A"
 
     definition player_tangle_attractor_I :: "'v set \<Rightarrow> bool" where
       "player_tangle_attractor_I S \<equiv> \<exists>\<sigma>.
@@ -545,15 +546,14 @@ begin
         \<and> (\<forall>x\<in>S. \<forall>xs ys. lasso_from_node (induced_subgraph V\<^sub>\<alpha> \<sigma>) x xs ys
             \<longrightarrow> (set (xs@ys) \<inter> A \<noteq> {} \<or> winning_player ys))"
 
-    lemma player_tangle_attractor_I_base[simp]:
+    lemma player_tangle_attractor_I_base:
       "player_tangle_attractor_I A"
       unfolding player_tangle_attractor_I_def
       apply (rule exI[where x="Map.empty"]; intro conjI; simp)
       using origin_in_lasso by fastforce
 
     lemma player_tangle_attractor_I_step:
-      "attractor_step S S' \<Longrightarrow> player_tangle_attractor_I S
-       \<Longrightarrow> player_tangle_attractor_I S'"
+      "attractor_step S S' \<Longrightarrow> player_tangle_attractor_I S \<Longrightarrow> player_tangle_attractor_I S'"
     proof (induction rule: attractor_step.induct)
       case (own x S y)
       from own.prems obtain \<sigma> where
@@ -566,13 +566,13 @@ begin
         unfolding player_tangle_attractor_I_def
         by auto
 
-      from own.hyps have new_strat: "strategy_of V\<^sub>\<alpha> (\<sigma> ++ [x\<mapsto>y])"
+      from own.hyps(1,2) have new_strat: "strategy_of V\<^sub>\<alpha> (\<sigma> ++ [x\<mapsto>y])"
         using strategy_of_add_same[OF \<sigma>_strat strategy_of_map_assign] by blast
 
-      from own.hyps \<sigma>_dom have new_dom: "dom (\<sigma> ++ [x\<mapsto>y]) = V\<^sub>\<alpha> \<inter> (insert x S - A)"
+      from own.hyps(1,4) \<sigma>_dom have new_dom: "dom (\<sigma> ++ [x\<mapsto>y]) = V\<^sub>\<alpha> \<inter> (insert x S - A)"
         by auto
 
-      from own.hyps \<sigma>_ran have new_ran: "ran (\<sigma> ++ [x\<mapsto>y]) \<subseteq> (insert x S)"
+      from own.hyps(3) \<sigma>_ran have new_ran: "ran (\<sigma> ++ [x\<mapsto>y]) \<subseteq> (insert x S)"
         unfolding ran_def by auto
 
       from \<sigma>_closed \<sigma>_ran own.hyps(1)
@@ -595,11 +595,9 @@ begin
           cycle_v'_ys: "cycle_node (induced_subgraph V\<^sub>\<alpha> (\<sigma> ++ [x\<mapsto>y])) v' ys"
           unfolding lasso_from_node_def by blast
 
-        show "set (xs@ys) \<inter> A \<noteq> {} \<or> winning_player ys"
-        proof (cases "set (xs@ys) \<inter> A \<noteq> {}")
-          case True thus ?thesis by simp
-        next
-          case False
+        have "set (xs@ys) \<inter> A = {} \<Longrightarrow> winning_player ys"
+        proof -
+          assume no_A: "set (xs@ys) \<inter> A = {}"
           hence xs_no_A: "set xs \<inter> A = {}" and ys_no_A: "set ys \<inter> A = {}" by auto
           with v_in_S' have v_in_S'_min_A: "v \<in> insert x S - A"
             using origin_in_lasso[OF lasso_v_xs_ys] by blast
@@ -610,14 +608,14 @@ begin
           from cycle_partially_closed_set[OF v'_in_S'_min_A new_closed cycle_v'_ys ys_no_A]
           have ys_in_S_min_A: "set ys \<subseteq> insert x S-A" by auto
 
-          have "lasso_from_node (induced_subgraph V\<^sub>\<alpha> \<sigma>) v' [] ys \<and> v'\<in>S"
-          proof (cases "x \<in> set ys")
-            case True
+          consider (ys_has_x) "x \<in> set ys" | (ys_no_x) "x \<notin> set ys" by blast
+          hence "lasso_from_node (induced_subgraph V\<^sub>\<alpha> \<sigma>) v' [] ys \<and> v'\<in>S" proof cases
+            case ys_has_x
             with own.hyps(1,2) obtain ys' where
               cycle_y_ys': "cycle_node (induced_subgraph V\<^sub>\<alpha> (\<sigma> ++ [x\<mapsto>y])) y ys'" and
               sets_eq: "set ys' = set ys" and
               y_in_ys': "y \<in> set ys'"
-              using cycle_node_intermediate_node[OF cycle_v'_ys True]
+              using cycle_node_intermediate_node[OF cycle_v'_ys ys_has_x]
               apply clarsimp
               subgoal for vs'
                 using cycle_node_D[of "induced_subgraph V\<^sub>\<alpha> (\<sigma> ++ [x\<mapsto>y])" x vs']
@@ -627,15 +625,15 @@ begin
             from own.hyps(3) sets_eq y_in_ys' ys_no_A have "y \<in> S-A" by blast
             from cycle_partially_closed_set[OF this new_closed_S cycle_y_ys'] sets_eq ys_no_A
             have "set ys \<subseteq> S - A" by simp
-            with True own.hyps(1) show ?thesis by blast
+            with ys_has_x own.hyps(1) show ?thesis by blast
           next
-            case False
+            case ys_no_x
             from own.hyps(1) have subset:
               "induced_subgraph V\<^sub>\<alpha> (\<sigma> ++ [x\<mapsto>y]) \<inter> (S-A)\<times>(S-A) \<subseteq> induced_subgraph V\<^sub>\<alpha> \<sigma>"
               unfolding induced_subgraph_def E_of_strat_def
               by (auto split: if_splits)
 
-            from False ys_in_S_min_A have ys_in_S_min_A: "set ys \<subseteq> S-A" by blast
+            from ys_no_x ys_in_S_min_A have ys_in_S_min_A: "set ys \<subseteq> S-A" by blast
             from subgraph_cycle[OF subset cycle_restr_V[OF cycle_v'_ys this]]
             have cycle_\<sigma>_v'_ys: " cycle_node (induced_subgraph V\<^sub>\<alpha> \<sigma>) v' ys " .
 
@@ -647,6 +645,7 @@ begin
           qed
           with \<sigma>_forces_A_or_wins ys_no_A show ?thesis by fastforce
         qed
+        thus "set (xs@ys) \<inter> A \<noteq> {} \<or> winning_player ys" by blast
       qed
 
       show ?case
@@ -665,11 +664,76 @@ begin
         \<sigma>_strat: "strategy_of V\<^sub>\<alpha> \<sigma>" and
         \<sigma>_dom: "dom \<sigma> = V\<^sub>\<alpha> \<inter> (S-A)" and
         \<sigma>_ran: "ran \<sigma> \<subseteq> S" and
-        \<sigma>_closed: "induced_subgraph V\<^sub>\<alpha> \<sigma> `` (S-A) \<subseteq> S" and
+        \<sigma>_closed_S: "induced_subgraph V\<^sub>\<alpha> \<sigma> `` (S-A) \<subseteq> S" and
         \<sigma>_forces_A_or_wins: "(\<forall>x\<in>S. \<forall>xs ys. lasso_from_node (induced_subgraph V\<^sub>\<alpha> \<sigma>) x xs ys
             \<longrightarrow> (set (xs@ys) \<inter> A \<noteq> {} \<or> winning_player ys))"
         unfolding player_tangle_attractor_I_def
         by auto
+
+      have \<sigma>_closed_S': "induced_subgraph V\<^sub>\<alpha> \<sigma> `` (insert x S - A) \<subseteq> insert x S"
+        using \<sigma>_closed_S opponent.hyps(2) by auto
+
+      have \<sigma>_forces_A_or_wins_S':
+        "\<forall>x\<in>insert x S. \<forall>xs ys. lasso_from_node (induced_subgraph V\<^sub>\<alpha> \<sigma>) x xs ys
+        \<longrightarrow> set (xs @ ys) \<inter> A \<noteq> {} \<or> winning_player ys"
+      proof (intro ballI allI impI)
+        fix v xs ys
+        assume v_in_S': "v \<in> insert x S" and
+               lasso_v_xs_ys: "lasso_from_node (induced_subgraph V\<^sub>\<alpha> \<sigma>) v xs ys"
+        from lasso_v_xs_ys obtain v' where
+          path_v_xs_v': "path (induced_subgraph V\<^sub>\<alpha> \<sigma>) v xs v'" and
+          cycle_v'_ys: "cycle_node (induced_subgraph V\<^sub>\<alpha> \<sigma>) v' ys"
+          unfolding lasso_from_node_def by blast
+
+        have "set (xs@ys) \<inter> A = {} \<Longrightarrow> winning_player ys"
+        proof -
+          assume no_A: "set (xs@ys) \<inter> A = {}"
+          hence xs_no_A: "set xs \<inter> A = {}" and ys_no_A: "set ys \<inter> A = {}" by auto
+          with v_in_S' have v_in_S'_min_A: "v \<in> insert x S - A"
+            using origin_in_lasso[OF lasso_v_xs_ys] by blast
+
+          from path_partially_closed_dest[OF v_in_S'_min_A \<sigma>_closed_S' path_v_xs_v' xs_no_A] ys_no_A
+          have v'_in_S'_min_A: "v' \<in> insert x S - A"
+            using origin_in_cycle_node[OF cycle_v'_ys] by blast
+          from cycle_partially_closed_set[OF this \<sigma>_closed_S' cycle_v'_ys ys_no_A]
+          have ys_in_S'_min_A: "set ys \<subseteq> insert x S - A" .
+
+          consider (ys_has_x) "x \<in> set ys" | (ys_no_x) "x \<notin> set ys" by blast
+          hence "lasso_from_node (induced_subgraph V\<^sub>\<alpha> \<sigma>) v' [] ys \<and> v' \<in> S" proof cases
+            case ys_has_x
+            with opponent.hyps(1,2) obtain y ys' where
+              x_y_edge: "(x,y) \<in> induced_subgraph V\<^sub>\<alpha> \<sigma>" and
+              y_in_S: "y \<in> S" and
+              cycle_y_ys': "cycle_node (induced_subgraph V\<^sub>\<alpha> \<sigma>) y ys'" and
+              sets_eq: "set ys' = set ys" and
+              y_in_ys': "y \<in> set ys'"
+              using cycle_node_intermediate_node[OF cycle_v'_ys ys_has_x]
+              apply clarsimp
+              subgoal for vs'
+                using cycle_node_D[of "induced_subgraph V\<^sub>\<alpha> (\<sigma>)" x vs']
+                using ind_subgraph_to_strategy by blast
+              done
+
+            from y_in_S y_in_ys' sets_eq ys_no_A have y_in_S_min_A: "y \<in> S-A" by blast
+            from cycle_partially_closed_set[OF this \<sigma>_closed_S cycle_y_ys'] sets_eq ys_no_A
+            have "set ys \<subseteq> S-A" by auto
+            hence "v' \<in> S"
+              using origin_in_cycle_node[OF cycle_v'_ys] by blast
+
+            with cycle_v'_ys show ?thesis
+              by (simp add: cycle_node_iff_loop loop_impl_lasso)
+          next
+            case ys_no_x
+            with ys_in_S'_min_A have ys_in_S_min_A: "set ys \<subseteq> S-A" by blast
+            with origin_in_cycle_node[OF cycle_v'_ys] have v'_in_S_min_A: "v' \<in> S-A" by blast
+            with cycle_v'_ys show ?thesis
+              by (simp add: cycle_node_iff_loop loop_impl_lasso)
+          qed
+
+          with \<sigma>_forces_A_or_wins no_A show ?thesis by fastforce
+        qed
+        thus "set (xs@ys) \<inter> A \<noteq> {} \<or> winning_player ys" by blast
+      qed
 
       show ?case
         unfolding player_tangle_attractor_I_def
@@ -677,15 +741,208 @@ begin
           subgoal using \<sigma>_strat .
           subgoal using \<sigma>_dom opponent.hyps(1) by force
           subgoal using \<sigma>_ran by auto
-          subgoal using \<sigma>_closed opponent.hyps(2) by auto
-          subgoal sorry
+          subgoal using \<sigma>_closed_S' .
+          subgoal using \<sigma>_forces_A_or_wins_S' .
         done
 
     next
       case (escape t S)
-      then show ?case sorry
+      from escape.prems obtain \<sigma> where
+        \<sigma>_strat: "strategy_of V\<^sub>\<alpha> \<sigma>" and
+        \<sigma>_dom: "dom \<sigma> = V\<^sub>\<alpha> \<inter> (S - A)" and
+        \<sigma>_ran: "ran \<sigma> \<subseteq> S" and
+        \<sigma>_closed_S: "induced_subgraph V\<^sub>\<alpha> \<sigma> `` (S - A) \<subseteq> S" and
+        \<sigma>_forces_A_or_wins: "\<forall>x\<in>S. \<forall>xs ys. lasso_from_node (induced_subgraph V\<^sub>\<alpha> \<sigma>) x xs ys
+          \<longrightarrow> set (xs @ ys) \<inter> A \<noteq> {} \<or> winning_player ys"
+        unfolding player_tangle_attractor_I_def by auto
+
+      from escape.hyps(1) have t_tangle: "player_tangle t" using tangles_T by simp
+
+      from t_tangle have
+        t_notempty: "t \<noteq> {}" and
+        t_in_V: "t \<subseteq> V"
+        using player_tangle_in_V by auto
+
+      from t_tangle obtain \<sigma>' where
+       \<sigma>'_strat: "strategy_of V\<^sub>\<alpha> \<sigma>'" and
+       \<sigma>'_dom: "dom \<sigma>' = t \<inter> V\<^sub>\<alpha>" and
+       \<sigma>'_ran: "ran \<sigma>' \<subseteq> t" and
+       \<sigma>'_strongly_connected_subgraph: "strongly_connected (player_tangle_subgraph t \<sigma>')" and
+       \<sigma>'_winning: "\<forall>v\<in>t. \<forall>xs. cycle_node (player_tangle_subgraph t \<sigma>') v xs \<longrightarrow> winning_player xs"
+        unfolding player_tangle_def is_player_tangle_strat_def Let_def by auto
+
+      define \<tau> where "\<tau> = (\<sigma>' |` (t-A)) ++ \<sigma>"
+      have \<tau>_strat: "strategy_of V\<^sub>\<alpha> \<tau>"
+      proof -
+        from \<sigma>'_strat have "strategy_of V\<^sub>\<alpha> (\<sigma>' |` (t-A))"
+          unfolding strategy_of_def E_of_strat_def
+          apply (simp; safe)
+            subgoal for x y by blast
+            subgoal for x y using restrict_in[of x "t-A" \<sigma>'] by fastforce
+          done
+          from strategy_of_add_same[OF this \<sigma>_strat] show ?thesis
+            unfolding \<tau>_def by blast
+      qed
+
+      from \<sigma>_dom \<sigma>'_dom have \<tau>_dom: "dom \<tau> =  V\<^sub>\<alpha> \<inter> (S \<union> t - A)"
+        unfolding \<tau>_def by auto
+
+      have \<tau>_ran: "ran \<tau> \<subseteq> S\<union>t"
+      proof -
+        have "ran (\<sigma>' |` (t-A)) \<subseteq> t"
+          using subsetD[OF \<sigma>'_ran] ran_restrictD[of _ \<sigma>' "t-A"] ranI by fast
+        with \<sigma>_ran show ?thesis
+          unfolding \<tau>_def ran_def by blast
+      qed
+
+      have \<tau>_closed_S: "induced_subgraph V\<^sub>\<alpha> \<tau> `` (S-A) \<subseteq> S"
+      proof (rule subsetI)
+        fix y assume y_succ: "y\<in>induced_subgraph V\<^sub>\<alpha> \<tau> `` (S-A)"
+        then obtain x where
+          x_y_edge: "(x,y)\<in>induced_subgraph V\<^sub>\<alpha> \<tau>" and
+          x_in_S_min_A: "x\<in>S-A"
+          by blast
+        consider (in_\<tau>) "x \<in> dom \<tau>" | (notin_\<tau>) "x \<notin> dom \<tau>" by blast
+        thus "y \<in> S" proof cases
+          case in_\<tau>
+          with \<tau>_dom have x_in_V\<^sub>\<alpha>: "x \<in> V\<^sub>\<alpha>" by simp
+          from ind_subgraph_to_strategy[OF x_y_edge x_in_V\<^sub>\<alpha>] have \<tau>_x_y: "\<tau> x = Some y" .
+
+          from x_in_V\<^sub>\<alpha> \<tau>_x_y \<sigma>_dom \<sigma>_ran x_in_S_min_A show ?thesis
+            unfolding \<tau>_def by (simp add: map_add_dom_app_simps(1) ranI subsetD)
+        next
+          case notin_\<tau>
+          with x_y_edge \<tau>_dom x_in_S_min_A
+          have x_y_edge_\<sigma>: "(x,y)\<in>induced_subgraph V\<^sub>\<alpha> \<sigma>"
+            using ind_subgraph_notin_dom by auto
+          with \<sigma>_closed_S x_in_S_min_A show ?thesis by blast
+        qed
+      qed
+
+      have \<tau>_closed_S': "induced_subgraph V\<^sub>\<alpha> \<tau> `` (S\<union>t-A) \<subseteq> S\<union>t"
+      proof (rule subsetI)
+        fix y assume y_succ: "y\<in>induced_subgraph V\<^sub>\<alpha> \<tau> `` (S\<union>t-A)"
+        then obtain x where
+          x_y_edge: "(x,y)\<in>induced_subgraph V\<^sub>\<alpha> \<tau>" and
+          x_in_S'_min_A: "x\<in>S\<union>t-A"
+          by blast
+
+        consider (in_\<tau>) "x \<in> dom \<tau>" | (notin_\<tau>) "x \<notin> dom \<tau>" by blast
+        thus "y\<in>S\<union>t" proof cases
+          case in_\<tau> with \<tau>_dom \<tau>_ran show ?thesis
+            using ind_subgraph_edge_dst[OF x_y_edge] by blast
+        next
+          case notin_\<tau>
+          consider (in_S_min_A) "x \<in> S-A" | (notin_S_min_A) "x \<notin> S-A" by blast
+          thus ?thesis proof cases
+            case in_S_min_A with x_y_edge \<tau>_closed_S show ?thesis by blast
+          next
+            case notin_S_min_A
+            with x_in_S'_min_A have x_in_t_min_A: "x \<in> t-A" by blast
+            thus ?thesis
+              apply (cases "y\<in>opponent_escapes t")
+                subgoal using escape.hyps(4) by blast
+                subgoal unfolding opponent_escapes_def
+                  using notin_\<tau> \<tau>_dom ind_subgraph_edge_in_E[OF x_y_edge] E_in_V
+                  by blast
+              done
+          qed
+        qed
+      qed
+
+      have \<tau>_forces_A_or_wins:
+        "\<forall>x\<in>S \<union> t. \<forall>xs ys. lasso_from_node (induced_subgraph V\<^sub>\<alpha> \<tau>) x xs ys
+          \<longrightarrow> set (xs @ ys) \<inter> A \<noteq> {} \<or> winning_player ys"
+      proof (intro ballI allI impI)
+        fix v xs ys
+        assume v_in_S': "v\<in>S\<union>t" and
+               lasso_v_xs_ys: "lasso_from_node (induced_subgraph V\<^sub>\<alpha> \<tau>) v xs ys"
+        from lasso_v_xs_ys obtain v' where
+          path_v_xs_v': "path (induced_subgraph V\<^sub>\<alpha> \<tau>) v xs v'" and
+          cycle_v'_ys: "cycle_node (induced_subgraph V\<^sub>\<alpha> \<tau>) v' ys"
+          unfolding lasso_from_node_def by blast
+
+        have "set (xs@ys) \<inter> A = {} \<Longrightarrow> winning_player ys"
+        proof -
+          assume no_A: "set (xs@ys) \<inter> A = {}"
+          hence xs_no_A: "set xs \<inter> A = {}" and ys_no_A: "set ys \<inter> A = {}" by auto
+          with v_in_S' have v_in_S'_min_A: "v\<in>(S\<union>t)-A"
+            using origin_in_lasso[OF lasso_v_xs_ys] by blast
+
+          from path_partially_closed_dest[OF v_in_S'_min_A \<tau>_closed_S' path_v_xs_v' xs_no_A] ys_no_A
+          have v'_in_S'_min_A: "v'\<in>(S\<union>t)-A" using origin_in_cycle_node[OF cycle_v'_ys] by blast
+          from cycle_partially_closed_set[OF v'_in_S'_min_A \<tau>_closed_S' cycle_v'_ys ys_no_A]
+          have ys_in_S'_min_A: "set ys \<subseteq> (S\<union>t)-A" .
+
+          from \<sigma>_dom have subset: "induced_subgraph V\<^sub>\<alpha> \<tau> \<inter> (S-A)\<times>(S-A) \<subseteq> induced_subgraph V\<^sub>\<alpha> \<sigma>"
+            unfolding \<tau>_def induced_subgraph_def E_of_strat_def
+            by auto
+
+          consider (ys_has_S) "set ys \<inter> S \<noteq> {}" | (ys_no_S) "set ys \<inter> S = {}" by blast
+          thus ?thesis proof cases
+            (** In this case, the cycle must be entirely contained in S because S is closed under
+                \<tau>. That also means it is won because under \<sigma>, all plays that do not go through A
+                are winning. *)
+            case ys_has_S
+            with ys_no_A obtain y ys' where
+              y_in_S_min_A: "y \<in> S-A" and
+              sets_eq: "set ys' = set ys" and
+              ys'_no_A: "set ys' \<inter> A = {}" and
+              cycle_y_ys': "cycle_node (induced_subgraph V\<^sub>\<alpha> \<tau>) y ys'"
+              using cycle_node_intermediate_node[OF cycle_v'_ys] by fastforce
+
+            from cycle_partially_closed_set[OF y_in_S_min_A \<tau>_closed_S cycle_y_ys' ys'_no_A] sets_eq
+            have ys_in_S_min_A: "set ys \<subseteq> S-A" by blast
+            hence v'_in_S: "v' \<in> S" using origin_in_cycle_node[OF cycle_v'_ys] by blast
+
+            from subgraph_cycle[OF subset cycle_restr_V[OF cycle_v'_ys ys_in_S_min_A]]
+            have "lasso_from_node (induced_subgraph V\<^sub>\<alpha> \<sigma>) v' [] ys"
+              by (simp add: cycle_node_iff_loop loop_impl_lasso)
+
+            with \<sigma>_forces_A_or_wins v'_in_S no_A show ?thesis by fastforce
+          next
+            case ys_no_S
+            with ys_in_S'_min_A have ys_in_t_min_S_min_A: "set ys \<subseteq> t-S-A" by blast
+            hence v'_in_t: "v'\<in>t" using origin_in_cycle_node[OF cycle_v'_ys] by blast
+
+            from \<sigma>_ran t_in_V have subset:
+              "induced_subgraph V\<^sub>\<alpha> \<tau> \<inter> (t-S-A)\<times>(t-S-A) \<subseteq> player_tangle_subgraph t \<sigma>' \<inter> (t-S-A)\<times>(t-S-A)"
+              unfolding \<tau>_def induced_subgraph_def player_tangle_subgraph_def E_of_strat_def
+              using ind_subgraph_edge_dst[of _ _ V\<^sub>\<alpha> \<sigma>] strategy_to_ind_subgraph[of \<sigma> _ _ V\<^sub>\<alpha>]
+              by fastforce
+
+            from subgraph_cycle[OF subset cycle_restr_V[OF cycle_v'_ys ys_in_t_min_S_min_A]]
+            have "cycle_node (player_tangle_subgraph t \<sigma>') v' ys" using restr_V_cycle by fast
+
+            with \<sigma>'_winning v'_in_t show ?thesis by blast
+          qed
+        qed
+        thus "set (xs@ys) \<inter> A \<noteq> {} \<or> winning_player ys" by blast
+      qed
+
+      show ?case
+        unfolding player_tangle_attractor_I_def
+        apply (rule exI[where x="\<tau>"]; intro conjI)
+          subgoal using \<tau>_strat .
+          subgoal using \<tau>_dom .
+          subgoal using \<tau>_ran .
+          subgoal using \<tau>_closed_S' .
+          subgoal using \<tau>_forces_A_or_wins .
+        done
     qed
+
+    (** I don't know if this is the correct name for this lemma. *)
+    lemma attractor_step_sound:
+      shows "attractor_step\<^sup>*\<^sup>* S S' \<Longrightarrow> player_tangle_attractor_I S \<Longrightarrow> player_tangle_attractor_I S'"
+      apply (induction rule: rtranclp_induct)
+        subgoal by blast
+        subgoal for X Y using player_tangle_attractor_I_step[of X Y] by blast
+      done
 end
+
+lemma "is_player_tangle_attractor A S \<Longrightarrow> player_tangle_attractor_I A S"
+  unfolding is_player_tangle_attractor_def
+  using player_tangle_attractor_I_base attractor_step_sound by blast
 
 lemma
   assumes "\<And>A A'. attractor_step A A'\<Longrightarrow> I A \<Longrightarrow> I A'"
